\documentclass[a4paper]{article}
\usepackage{amsmath}
\usepackage{amssymb}
\usepackage[ngerman]{babel}
\title{Computergrafik}
\author{Lisa Kassebaum - 199856 \\ Andreas Pfohl \\ Martin Knoll - 193321 }
\date{}
\begin{document}
\maketitle
\section{}
\subsection{}
  \begin{align*}
    \left|v\right|
    =
    \left|
    \begin{pmatrix}
      1 \\ 4 \\ 3
    \end{pmatrix}
    \right|
    =
    \sqrt{1^2 + 4^2 + 3^2}
    = \sqrt{26} &=& 5,1
    \\[1em]
    v\text{ normalisiert}: \quad \frac{1}{\sqrt{26}} = 0,2 \quad \frac{4}{\sqrt{26}} = 0,78 \quad \frac{3}{\sqrt{26}} = 0,58
    \\[1em]
    \left|v\text{ normalisiert}\right|: \quad \sqrt{0,2^2 + 0,78^2 + 0,58^2} &=& 1
  \end{align*}

  \begin{align*}
    \left|v\right|
    =
    \left|
    \begin{pmatrix}
      0 \\ 0 \\ 12
    \end{pmatrix}
    \right|
    =
    \sqrt{0^2 + 0^2 + 12^2}
    = \sqrt{144} &=& 12
    \\[1em]
    v\text{ normalisiert}: \quad \frac{0}{\sqrt{12}} = 0 \quad \frac{0}{\sqrt{12}} = 0 \quad \frac{12}{\sqrt{12}} = 1
    \\[1em]
    \left|v\text{ normalisiert}\right|: \quad \sqrt{0^2 + 0^2 + 1^2} &=& 1
  \end{align*}

  \begin{align*}
    \left|v\right|
    =
    \left|
    \begin{pmatrix}
      -2 \\ 0 \\ 1
    \end{pmatrix}
    \right|
    =
    \sqrt{(-2)^2 + 0^2 + 1^2}
    = \sqrt{5} &=& 2,24
    \\[1em]
    v\text{ normalisiert}: \quad \frac{-2}{\sqrt{5}} = -0,89 \quad \frac{0}{\sqrt{5}} = 0 \quad \frac{1}{\sqrt{5}} = 0,45
    \\[1em]
    \left|v\text{ normalisiert}\right|: \quad \sqrt{(-0,2)^2 + 0^2 + 0,45^2} &=& 1
  \end{align*}

\subsection{}
  \begin{align*}
    \begin{pmatrix}
      1 \\ 4 \\ 7
    \end{pmatrix}
    \times
    \begin{pmatrix}
      -2 \\ 0 \\ 3
    \end{pmatrix}
    &=& 19
    \\[1em]
    \begin{pmatrix}
      -5 \\ 1 \\ 3
    \end{pmatrix}
    \times
    \begin{pmatrix}
      4 \\ -2 \\ 1
    \end{pmatrix}
    &=& -19
    \\[1em]
    \begin{pmatrix}
      -5 \\ 1 \\ 3
    \end{pmatrix}
    \times
    \begin{pmatrix}
      4 \\ -2 \\ 1
    \end{pmatrix}
    &=& 0
  \end{align*}
\subsection{}
  \begin{align*}
    \begin{pmatrix}
      5 \\ 3 \\ 0
    \end{pmatrix}
    \times
    \begin{pmatrix}
      -2 \\ 4 \\ 0
    \end{pmatrix}
    &=&
    \begin{pmatrix}
      0 \\ 0 \\ 26
    \end{pmatrix}
    \\[1em]
    \begin{pmatrix}
      1 \\ 0 \\ 0
    \end{pmatrix}
    \times
    \begin{pmatrix}
      0 \\ 1 \\ 1
    \end{pmatrix}
    &=&
    \begin{pmatrix}
      0 \\ -1 \\ 1
    \end{pmatrix}
  \end{align*}
  \subsection{}
    \begin{align*}
      c = \vec{a} \times \vec{b}
      =
      \begin{pmatrix}
      a_1 \\ a_2 \\ a_3
      \end{pmatrix}
      \times
      \begin{pmatrix}
      b_1 \\ b_2 \\ b_3
      \end{pmatrix}
      =
      \begin{pmatrix}
      a_2 b_3 - a_3 b_2 \\ a_3 b_1 - a_1 b_3 \\ a_1 b_2 - a_2 b_1
      \end{pmatrix}
      \\[1em]
      \vec{c} \cdot \vec{a}
      =
      \begin{pmatrix}
      a_2 b_3 - a_3 b_2 \\ a_3 b_1 - a_1 b_3 \\ a_1 b_2 - a_2 b_1
      \end{pmatrix}
      \begin{pmatrix}
      a_1 \\ a_2 \\ a_3
      \end{pmatrix}
      \\[1em]
      = (a_2 b_3 - a_3 b_1) (a_1) + (a_3 b_1 - a_1 b_3) (a_2) + (a_1 b_2 - a_2 b_1) (a_3)
      \\[1em]
      = a_1 a_2 b_3 - a_1 a_3 b_2 + a_2 a_3 b_1 - a_1 a_2 b_3 + a_1 a_3 b_2 - a_2 a_3 b_1
      = 0
      \\[1em]
      \vec{c} \cdot \vec{b}
      =
      \begin{pmatrix}
      a_2 b_3 - a_3 b_2 \\ a_3 b_1 - a_1 b_3 \\ a_1 b_2 - a_2 b_1
      \end{pmatrix}
      \begin{pmatrix}
      b_1 \\ b_2 \\ b_3
      \end{pmatrix}
      \\[1em]
      = (a_2 b_3 - a_3 b_1) (b_1) + (a_3 b_1 - a_1 b_3) (b_2) + (a_1 b_2 - a_2 b_1) (b_3)
      \\[1em]
      = a_2 b_1 b_3 - a_3 b_1 b_2 + a_3 b_1 b_2 - a_1 b_2 b_3 + a_1 b_3 b_2 - a_2 b_1 b_3
      = 0
    \end{align*}
\end{document}
